logic/logic_tactics.v
@@ -1,0 +1,100 @@
+Add LoadPath "???\syntax".
+Add LoadPath "???\type_system".
+Add LoadPath "???\substitution".
+Add LoadPath "???\operational_semantics".
+Add LoadPath "???\logic".
+
+Require Export type_lemmas.
+
+
+Ltac simpl_c_subs := 
+unfold c_subs2_out; unfold c_subs_out; unfold c_subs; simpl.
+
+Ltac obvious := 
+   apply WfCtxØ || (apply WfCtxU; obvious) 
+|| apply WfTCtxØ  || (apply WfTCtxU; obvious) 
+|| apply WfEqsØ || apply WfSigØ || (apply WfSigU; obvious)
+|| apply WfTyUnit || apply WfTyInt || apply WfTyEmpty
+|| (apply WfTyHandler; obvious) || (apply WfTyFun; obvious) 
+|| (apply WfTyList; obvious)|| (apply WfTySum; obvious)
+|| (apply WfTyProd; obvious) || (apply WfCTy; obvious)
+|| auto.
+
+Ltac obvious_vtype := (
+(apply TypeV; (
+   (apply TypeUnit; obvious)
+|| (apply TypeInt; obvious)
+|| (apply TypeLeft; obvious_vtype)
+|| (apply TypeRight; obvious_vtype)
+|| (apply TypePair; obvious_vtype)
+|| (apply TypeNil; obvious)
+|| (apply TypeFun; obvious)
+|| (apply TypeCons; obvious_vtype)
+|| (apply TypeVar; simpl in *; obvious)
+|| obvious)
+)
+|| obvious).
+
+Ltac vtype_step := (
+(apply TypeV; (
+   (apply TypeUnit; obvious)
+|| (apply TypeInt; obvious)
+|| (apply TypeLeft; obvious)
+|| (apply TypeRight; obvious)
+|| (apply TypePair; obvious)
+|| (apply TypeNil; obvious)
+|| (apply TypeCons; obvious)
+|| (apply TypeFun; obvious)
+|| (apply TypeHandler; obvious)
+|| (apply TypeVar; simpl in *; obvious)
+|| obvious)
+)
+|| obvious).
+
+
+Ltac obvious_ctype := (
+(apply TypeC; (
+  (apply TypeRet; obvious_vtype)
+|| (eapply TypeApp; obvious_vtype)
+|| (eapply TypeOp; ((apply vsubtype_refl; obvious) || obvious_vtype || auto))
+|| (eapply TypeSumMatch; obvious_vtype; obvious_ctype)
+|| (eapply TypeProdMatch; obvious_vtype; obvious_ctype)
+|| (eapply TypeListMatch; obvious_vtype; obvious_ctype)
+|| obvious)
+)
+|| obvious).
+
+Ltac ctype_step := (
+(apply TypeC; (
+  (apply TypeRet; obvious)
+|| (eapply TypeApp; obvious)
+|| (eapply TypeSumMatch; obvious)
+|| (eapply TypeProdMatch; obvious)
+|| (eapply TypeListMatch; obvious)
+|| (eapply TypeDo; obvious)
+|| (eapply TypeLetRec; obvious)
+|| obvious)
+)
+|| obvious).
+
+Ltac wft_step := (
+   (eapply WfTApp; obvious)
+|| (eapply WfTSumMatch; obvious)
+|| (eapply WfTProdMatch; obvious)
+|| (eapply WfTListMatch; obvious)
+|| (eapply WfTDo; obvious)
+|| (eapply WfTOp; obvious)
+|| obvious).
+
+
+
+Lemma dirty_ret Γ A Σ E v:
+  wf_sig Σ -> wf_eqs E Σ -> has_vtype Γ v A ->
+  has_ctype Γ (Ret v) (CTy A Σ E).
+Proof.
+intros wfs wfe vty. apply TypeC. inv vty. auto. obvious. inv vty. auto.
+eapply TypeCSubsume. instantiate (1:= (CTy A SigØ EqsØ)).
+obvious_ctype. all: inv vty; auto. apply STyCTy.
+apply vsubtype_refl. auto. apply STySigØ. apply STyEqsØ.
+Qed.
+
