type_system/instantiation_lemmas.v
@@ -1,11 +1,7 @@
-(* Add LoadPath "C:\Users\Ziga\Documents\Ziga_podatki\repositories\eeff-formalization\syntax". *)
-(* Add LoadPath "C:\Users\Ziga\Documents\Ziga_podatki\repositories\eeff-formalization\type_system". *)
-(* Add LoadPath "C:\Users\Ziga\Documents\Ziga_podatki\repositories\eeff-formalization\substitution". *)
-(* Add LoadPath "C:\Users\Ziga\Documents\Ziga_podatki\repositories\eeff-formalization\logic". *)
-Add LoadPath "E:\Ziga_Podatki\faks\eeff-formalization\syntax".
-Add LoadPath "E:\Ziga_Podatki\faks\eeff-formalization\type_system".
-Add LoadPath "E:\Ziga_Podatki\faks\eeff-formalization\substitution".
-Add LoadPath "E:\Ziga_Podatki\faks\eeff-formalization\logic".
+Add LoadPath "???\syntax".
+Add LoadPath "???\type_system".
+Add LoadPath "???\substitution".
+Add LoadPath "???\logic".
 
 Require Export subtyping_lemmas substitution_lemmas type_aux_lemmas.
 
