type_system/type_lemmas.v
@@ -1,13 +1,8 @@
-(* Add LoadPath "C:\Users\Ziga\Documents\Ziga_podatki\repositories\eeff-formalization\syntax". *)
-(* Add LoadPath "C:\Users\Ziga\Documents\Ziga_podatki\repositories\eeff-formalization\substitution". *)
-(* Add LoadPath "C:\Users\Ziga\Documents\Ziga_podatki\repositories\eeff-formalization\type_system". *)
-(* Add LoadPath "C:\Users\Ziga\Documents\Ziga_podatki\repositories\eeff-formalization\operational_semantics". *)
-(* Add LoadPath "C:\Users\Ziga\Documents\Ziga_podatki\repositories\eeff-formalization\logic". *)
-Add LoadPath "E:\Ziga_Podatki\faks\eeff-formalization\syntax".
-Add LoadPath "E:\Ziga_Podatki\faks\eeff-formalization\substitution".
-Add LoadPath "E:\Ziga_Podatki\faks\eeff-formalization\type_system".
-Add LoadPath "E:\Ziga_Podatki\faks\eeff-formalization\operational_semantics".
-Add LoadPath "E:\Ziga_Podatki\faks\eeff-formalization\logic".
+Add LoadPath "???\syntax".
+Add LoadPath "???\substitution".
+Add LoadPath "???\type_system".
+Add LoadPath "???\operational_semantics".
+Add LoadPath "???\logic".
 Require Export type_aux_lemmas operational_semantics.
 
 (* ==================== Substitution Lemma ==================== *)
